Prove per-function O1 structural outputs

venom/props/venomPipelineRunnerPropsScript.sml
@@ -3,6 +3,7 @@
 Theory venomPipelineRunnerProps
 Ancestors
   venomPipelineRunner venomFnScheduleRunnerProps fcgPostorder
+  venomPassDispatcherProps fmpLowerProps venomPassSchedule
 
 Theorem run_named_fn_schedules_append:
   run_named_fn_schedules runner rpolicy passes (xs ++ ys) unit supply =
@@ -216,4 +217,258 @@ Proof
   gvs[run_callee_first_def] >>
   metis_tac[run_named_fn_schedules_indexed]
 QED
+Theorem fmp_lower_function_success_no_raw[local]:
+  fmp_lower_function ctx s fn = SOME (fn',s') ==>
+  no_raw_fmp_ops fn'
+Proof
+  simp[fmpLowerDefsTheory.fmp_lower_function_def] >>
+  Cases_on `analyze_fmp_context ctx` >> simp[] >>
+  rename1 `analyze_fmp_context ctx = SOME infos` >>
+  Cases_on `fn.fn_fmp_signature`
+  >- (strip_tac >>
+      `fmp_lower_input infos ctx fn` by
+        (qpat_x_assum `fmp_lower_function_with_info _ _ _ _ = SOME _`
+          mp_tac >>
+         simp[fmpLowerDefsTheory.fmp_lower_function_with_info_def,
+              AllCaseEqs()]) >>
+      `fmp_lower_function ctx s fn = SOME (fn',s')` by
+        simp[fmpLowerDefsTheory.fmp_lower_function_def] >>
+      metis_tac[fmp_lower_function_removes_raw_ops]) >>
+  gvs[fmpLowerDefsTheory.fmp_lower_function_with_info_def,AllCaseEqs()] >>
+  rpt strip_tac >> gvs[]
+QED
+
+Definition o1_fn_structural_output_def[local]:
+  o1_fn_structural_output fn <=>
+    IS_SOME fn.fn_eom /\ no_raw_fmp_ops fn /\
+    IS_SOME fn.fn_fmp_signature
+End
+
+Theorem run_configured_fn_pass_fold_first_step[local]:
+  run_configured_fn_pass_fold execute_configured_fn_pass rpolicy
+    (pass::passes) unit s fn labels = SOME result ==>
+  ?out.
+    execute_configured_fn_pass rpolicy pass unit s fn = SOME out /\
+    fn_pass_effects_hold (fn_pass_tag pass) fn out /\
+    run_configured_fn_pass_fold execute_configured_fn_pass rpolicy
+      passes unit out.fpo_supply out.fpo_function
+      (labels ++ out.fpo_label_map) = SOME result
+Proof
+  simp[venomFnScheduleRunnerTheory.run_configured_fn_pass_fold_def] >>
+  Cases_on `execute_configured_fn_pass rpolicy pass unit s fn` >> simp[] >>
+  Cases_on `x.fpo_function.fn_name = fn.fn_name /\
+            fn_pass_effects_hold (fn_pass_tag pass) fn x /\
+            introduces_no_invoke_edges fn x.fpo_function /\
+            ir_supply_extends s x.fpo_supply /\
+            ir_supply_covers_fn x.fpo_supply x.fpo_function /\
+            ir_supply_covers_unit x.fpo_supply unit` >> simp[] >>
+  metis_tac[]
+QED
+
+Theorem execute_configured_fn_pass_o1_suffix_structural[local]:
+  MEM tag [VP_MakeSSA; VP_SimplifyCFG; VP_SingleUseExpansion;
+           VP_DFT; VP_CFGNormalization] /\
+  o1_fn_structural_output fn /\
+  execute_configured_fn_pass rpolicy (CFP_Simple tag) unit s fn = SOME out /\
+  fn_pass_effects_hold (fn_pass_tag (CFP_Simple tag)) fn out ==>
+  o1_fn_structural_output out.fpo_function
+Proof
+  rpt strip_tac >>
+  `no_raw_fmp_ops fn` by
+    fs[o1_fn_structural_output_def] >>
+  `no_raw_fmp_ops out.fpo_function` by
+    (irule execute_configured_fn_pass_o1_suffix_no_raw_fmp_ops >>
+     qexistsl [`fn`,`rpolicy`,`s`,`tag`,`unit`] >>
+     simp[]) >>
+  Cases_on `tag` >>
+  gvs[o1_fn_structural_output_def,
+      venomPassScheduleTheory.fn_pass_tag_def,
+      venomPassDispatcherTheory.fn_pass_effects_hold_def,
+      venomPassDispatcherTheory.fn_static_layout_effect_holds_def,
+      venomPassDispatcherTheory.fn_abi_effect_holds_def,
+      venomPassDispatcherTheory.fn_pass_static_layout_effect_def,
+      venomPassDispatcherTheory.fn_pass_abi_effect_def,
+      venomInstTheory.fn_static_layout_eq_def,
+      venomInstTheory.fn_fmp_convention_eq_def]
+QED
+
+Theorem subst_label_map_blocks_opcode_every[local]:
+  EVERY (\inst. P inst.inst_opcode)
+    (fn_insts_blocks (MAP (subst_label_map_block label_map) blocks)) <=>
+  EVERY (\inst. P inst.inst_opcode) (fn_insts_blocks blocks)
+Proof
+  Induct_on `blocks` >>
+  simp[venomInstTheory.fn_insts_blocks_def,
+       cfgTransformTheory.subst_label_map_block_def,
+       cfgTransformTheory.subst_label_map_inst_def,
+       listTheory.EVERY_APPEND, listTheory.EVERY_MAP]
+QED
+
+Theorem subst_label_map_fn_o1_structural[local]:
+  o1_fn_structural_output fn ==>
+  o1_fn_structural_output (subst_label_map_fn label_map fn)
+Proof
+  simp[o1_fn_structural_output_def,
+       venomInstTheory.no_raw_fmp_ops_def,
+       venomInstTheory.fn_insts_def,
+       cfgTransformTheory.subst_label_map_fn_def] >>
+  strip_tac >>
+  fs[GSYM listTheory.EVERY_MEM, subst_label_map_blocks_opcode_every]
+QED
+
+Theorem filter_subst_label_map_fn_name[local]:
+  FILTER (\fn. fn.fn_name = name)
+    (MAP (subst_label_map_fn label_map) fns) =
+  MAP (subst_label_map_fn label_map)
+    (FILTER (\fn. fn.fn_name = name) fns)
+Proof
+  Induct_on `fns`
+  >- simp[]
+  >> simp[cfgTransformTheory.subst_label_map_fn_def] >>
+  gen_tac >> Cases_on `h.fn_name = name` >>
+  simp[cfgTransformTheory.subst_label_map_fn_def]
+QED
+
+Theorem lookup_unique_function_subst_label_map[local]:
+  lookup_unique_function name fns = SOME fn ==>
+  lookup_unique_function name (MAP (subst_label_map_fn label_map) fns) =
+    SOME (subst_label_map_fn label_map fn)
+Proof
+  strip_tac >>
+  drule lookup_unique_function_FILTER >>
+  simp[venomFnScheduleRunnerTheory.lookup_unique_function_def,
+       filter_subst_label_map_fn_name]
+QED
+
+Theorem apply_unit_label_map_o1_lookup[local]:
+  apply_unit_label_map label_map unit = SOME unit' ==>
+  lookup_unique_function name unit.cu_context.ctx_functions = SOME fn ==>
+  o1_fn_structural_output fn ==>
+  ?fn'. lookup_unique_function name unit'.cu_context.ctx_functions = SOME fn' /\
+        o1_fn_structural_output fn'
+Proof
+  rpt strip_tac >>
+  qpat_x_assum `apply_unit_label_map label_map unit = SOME unit'` mp_tac >>
+  simp[unitLabelMapTheory.apply_unit_label_map_def] >>
+  Cases_on `resolve_label_map label_map` >> simp[] >>
+  Cases_on `resolved_label_endpoints_valid unit x` >> simp[] >>
+  strip_tac >>
+  gvs[unitLabelMapTheory.apply_resolved_unit_label_map_def] >>
+  qexists `subst_label_map_fn x fn` >>
+  simp[lookup_unique_function_subst_label_map,
+       subst_label_map_fn_o1_structural]
+QED
+
+Theorem run_o1_fn_pass_fold_structural[local]:
+  run_configured_fn_pass_fold execute_configured_fn_pass rpolicy
+    o1_fn_passes unit s fn labels = SOME result ==>
+  o1_fn_structural_output (FST result)
+Proof
+  strip_tac >>
+  qpat_x_assum
+    `run_configured_fn_pass_fold execute_configured_fn_pass rpolicy
+       o1_fn_passes unit s fn labels = SOME result`
+    (fn th => mp_tac (REWRITE_RULE [o1_fn_passes_def] th)) >>
+  strip_tac >>
+  dxrule run_configured_fn_pass_fold_first_step >> strip_tac >>
+  rename1 `execute_configured_fn_pass rpolicy (CFP_Simple VP_MakeSSA)
+             unit s fn = SOME out1` >>
+  dxrule run_configured_fn_pass_fold_first_step >> strip_tac >>
+  rename1 `execute_configured_fn_pass rpolicy (CFP_Simple VP_LowerDload)
+             unit out1.fpo_supply out1.fpo_function = SOME out2` >>
+  dxrule run_configured_fn_pass_fold_first_step >> strip_tac >>
+  rename1 `execute_configured_fn_pass rpolicy (CFP_Simple VP_ConcretizeMemLoc)
+             unit out2.fpo_supply out2.fpo_function = SOME out3` >>
+  dxrule run_configured_fn_pass_fold_first_step >> strip_tac >>
+  rename1 `execute_configured_fn_pass rpolicy (CFP_Simple VP_FmpLowering)
+             unit out3.fpo_supply out3.fpo_function = SOME out4` >>
+  `IS_SOME out3.fpo_function.fn_eom` by
+    gvs[venomPassScheduleTheory.fn_pass_tag_def,
+        venomPassDispatcherTheory.fn_pass_effects_hold_def,
+        venomPassDispatcherTheory.fn_static_layout_effect_holds_def,
+        venomPassDispatcherTheory.fn_pass_static_layout_effect_def] >>
+  `IS_SOME out4.fpo_function.fn_eom /\
+   IS_SOME out4.fpo_function.fn_fmp_signature` by
+    gvs[venomPassScheduleTheory.fn_pass_tag_def,
+        venomPassDispatcherTheory.fn_pass_effects_hold_def,
+        venomPassDispatcherTheory.fn_static_layout_effect_holds_def,
+        venomPassDispatcherTheory.fn_abi_effect_holds_def,
+        venomPassDispatcherTheory.fn_pass_static_layout_effect_def,
+        venomPassDispatcherTheory.fn_pass_abi_effect_def,
+        venomInstTheory.fn_static_layout_eq_def] >>
+  `no_raw_fmp_ops out4.fpo_function` by
+    (Cases_on
+       `fmp_lower_function unit.cu_context out3.fpo_supply out3.fpo_function` >>
+     gvs[] >> PairCases_on `x` >> gvs[] >>
+     metis_tac[fmp_lower_function_success_no_raw]) >>
+  `o1_fn_structural_output out4.fpo_function` by
+    simp[o1_fn_structural_output_def] >>
+  dxrule run_configured_fn_pass_fold_first_step >> strip_tac >>
+  rename1 `execute_configured_fn_pass rpolicy (CFP_Simple VP_MakeSSA)
+             unit out4.fpo_supply out4.fpo_function = SOME out5` >>
+  `o1_fn_structural_output out5.fpo_function` by
+    (irule execute_configured_fn_pass_o1_suffix_structural >>
+     qexistsl [`out4.fpo_function`,`rpolicy`,`out4.fpo_supply`,
+               `VP_MakeSSA`,`unit`] >> simp[venomPassScheduleTheory.fn_pass_tag_def]) >>
+  dxrule run_configured_fn_pass_fold_first_step >> strip_tac >>
+  rename1 `execute_configured_fn_pass rpolicy (CFP_Simple VP_SimplifyCFG)
+             unit out5.fpo_supply out5.fpo_function = SOME out6` >>
+  `o1_fn_structural_output out6.fpo_function` by
+    (irule execute_configured_fn_pass_o1_suffix_structural >>
+     qexistsl [`out5.fpo_function`,`rpolicy`,`out5.fpo_supply`,
+               `VP_SimplifyCFG`,`unit`] >> simp[venomPassScheduleTheory.fn_pass_tag_def]) >>
+  dxrule run_configured_fn_pass_fold_first_step >> strip_tac >>
+  rename1 `execute_configured_fn_pass rpolicy (CFP_Simple VP_SingleUseExpansion)
+             unit out6.fpo_supply out6.fpo_function = SOME out7` >>
+  `o1_fn_structural_output out7.fpo_function` by
+    (irule execute_configured_fn_pass_o1_suffix_structural >>
+     qexistsl [`out6.fpo_function`,`rpolicy`,`out6.fpo_supply`,
+               `VP_SingleUseExpansion`,`unit`] >> simp[venomPassScheduleTheory.fn_pass_tag_def]) >>
+  dxrule run_configured_fn_pass_fold_first_step >> strip_tac >>
+  rename1 `execute_configured_fn_pass rpolicy (CFP_Simple VP_DFT)
+             unit out7.fpo_supply out7.fpo_function = SOME out8` >>
+  `o1_fn_structural_output out8.fpo_function` by
+    (irule execute_configured_fn_pass_o1_suffix_structural >>
+     qexistsl [`out7.fpo_function`,`rpolicy`,`out7.fpo_supply`,
+               `VP_DFT`,`unit`] >> simp[venomPassScheduleTheory.fn_pass_tag_def]) >>
+  dxrule run_configured_fn_pass_fold_first_step >> strip_tac >>
+  rename1 `execute_configured_fn_pass rpolicy (CFP_Simple VP_CFGNormalization)
+             unit out8.fpo_supply out8.fpo_function = SOME out9` >>
+  `o1_fn_structural_output out9.fpo_function` by
+    (irule execute_configured_fn_pass_o1_suffix_structural >>
+     qexistsl [`out8.fpo_function`,`rpolicy`,`out8.fpo_supply`,
+               `VP_CFGNormalization`,`unit`] >> simp[venomPassScheduleTheory.fn_pass_tag_def]) >>
+  gvs[venomFnScheduleRunnerTheory.run_configured_fn_pass_fold_def]
+QED
+
+Theorem run_configured_fn_passes_o1_structural:
+  run_configured_fn_passes execute_configured_fn_pass rpolicy o1_fn_passes
+    name unit s = SOME (unit',s') ==>
+  ?fn'.
+    lookup_unique_function name unit'.cu_context.ctx_functions = SOME fn' /\
+    IS_SOME fn'.fn_eom /\ no_raw_fmp_ops fn' /\
+    IS_SOME fn'.fn_fmp_signature
+Proof
+  simp[venomFnScheduleRunnerTheory.run_configured_fn_passes_def] >>
+  strip_tac >> gvs[AllCaseEqs()] >>
+  `o1_fn_structural_output fn'` by
+    (drule run_o1_fn_pass_fold_structural >> simp[]) >>
+  `lookup_unique_function name fns = SOME fn'` by
+    (drule replace_unique_function_exactly_one >>
+     simp[venomFnScheduleRunnerTheory.lookup_unique_function_def]) >>
+  `apply_unit_label_map label_map
+      (unit with cu_context := unit.cu_context with ctx_functions := fns) =
+        SOME unit' /\
+   lookup_unique_function name fns = SOME fn' /\
+   o1_fn_structural_output fn'` by simp[] >>
+  `lookup_unique_function name
+      (unit with cu_context := unit.cu_context with ctx_functions := fns).
+        cu_context.ctx_functions = SOME fn' /\
+   o1_fn_structural_output fn'` by simp[] >>
+  drule apply_unit_label_map_o1_lookup >>
+  disch_then drule >> (impl_tac >- simp[]) >> strip_tac >>
+  goal_assum $ drule_at Any >>
+  gvs[o1_fn_structural_output_def]
+QED
+
 val _ = export_theory ();
